\section{Macroeconomics Final 2015 / 16}

{
\subsection*{Exercise 1}

\begin{enumerate}[label=(\arabic*)]
{\item 
$$
\begin{aligned}
Y_{t}(i) & =C_{t}(i)+\gamma_{t} Y_{t}(i) \\
\left(1-\gamma_{t}\right) Y_{t}(i) & =C_{t}(i) \\
\left(1-\gamma_{t}\right) \int_{0}^1 Y_{t}(i) d i & =\int_{0}^1 C_{t}(i) d i \\
\left(1-\gamma_{t}\right) Y_{t} & =C_{t} \\
\ln \left(1-\gamma_{t}\right)+y_{t} & =c_{t} \\
y_{t} & =c_{t}-\ln \left(1-\gamma_{t}\right)=c_{t}-g_{t}
\end{aligned}
$$
}
{
\item 

Optimality conditions of household are unchanged as $G_{t}(i)$ is financed via lump-sum:

$$
\begin{aligned}
C_{t}(i) & =\left(\frac{P_{t}(i)}{P_{t}}\right)^{-\varepsilon} C_{t} \\
Q_{t} & =\mathbb{E}_{t}\left[\frac{C_{t}}{C_{t+1}} \frac{P_{t}}{P_{t+1}}\right] \\
C_{t} N_{t}^{\varphi} & =\frac{W_{t}}{P_{t}} \\
\frac{M_{t}}{P_{t}} & =C_{t}\left[1-\exp \left(-i_{t}\right)\right]^{-1}=\left(Y_{t}-G_{t}\right)\left[1-\exp \left(-i_{t}\right)\right]^{-1}
\end{aligned}
$$

Since $Y_{t}$ increases in $N_{t}$, we have that a higher $G_{t}$ must increase employment. \color{red} Or $C_{t}$ goes down? \color{black}

Firms' pricing: (Assume $Y_{t}(i)=N_{t}(i)$ )

$$
\max _{P_{t}(i)} \mathbb{E}_{t-1}\left[\Lambda_{t-1, t} \frac{Y_{t}(i)}{P_{t}}\left(P_{t}(i)-W_{t}\right)\right]
$$

Use the market clearing condition: $Y_{t}(i)=C_{t}(i)+G_{t}(i)$

$$
\begin{aligned}
& \max _{P_{t}(i)} \mathbb{E}_{t-1}\left[\Lambda_{t-1, t} \frac{C_{t}(i)+G_{t}(i)}{P_{t}}\left(P_{t}(i)-W_{t}\right)\right] \\
& \max _{P_{t}(i)} \mathbb{E}_{t-1}\left[\Lambda_{t-1, t}\left(\frac{1}{P_{t}}\left(\frac{P_{t}(i)}{P_{t}}\right)^{-\varepsilon} C_{t}+\frac{G_{t}(i)}{P_{t}}\right)\left(P_{t}(i)-W_{t}\right)\right]
\end{aligned}
$$

$$
\max _{P_{t}(i)}\mathbb{E}_{t-1}\left[\Lambda_{t-1, t}\left(\frac{1}{P_{t}}\left(\frac{P_{t}(i)}{P_{t}}\right)^{-\varepsilon}\left(Y_{t}-G_{t}\right)+\frac{G_{t}(i)}{P_{t}}\right)\left(P_{t}(i)-W_{t}\right)\right]
$$

FOC:

\begin{align*}
\mathbb{E}_{t-1}\left[\Lambda_{t-1, t} \frac{1}{P_{t}^{1-\varepsilon}}(1-\varepsilon) P_{t}(i)^{-\varepsilon}\left(Y_{t}-G_{t}\right)\left(1-P_{t}(i)^{-1}(-\varepsilon) W_{t}\right)+\frac{G_{t}(i)}{P_{t}(1-\varepsilon)}\right] &= 0 \\
\mathbb{E}_{t-1}\left[\Lambda_{t-1, t}\underbrace{\left(\frac{P_t(i)}{P_t}\right)^{-\varepsilon} \frac{\left(Y_t-G_t\right)}{P_t}}_{\frac{Y_t(i)-G_t(i)}{P_t}}\left(1-P_t(i)^{-1} M W_t\right)+\frac{G_t(i)}{P_t(1-\varepsilon)}\right] &= 0 \\
\mathbb{E}_{t-1}\left[\Lambda_{t-1, t} \frac{Y_{t}(i)-G_{t}(i)}{P_{t}}\left(P_{t}(i)-M W_{t}\right)+\frac{G_{t}(i)}{P_{t}(1-\varepsilon)}\right] &= 0
\end{align*}


Impose symmetry: $Y_{t}(i)=Y_{t}$ and $P_{t}(i)=P_{t} \quad \forall i$

$$
\longrightarrow G_{t}(i)=G_{t} \text { and } G_{t}(i)=C_{t}
$$

$$
\mathbb{E}_{t-1}\left[\Lambda_{t-1, t}\left(Y_{t}-G_{t}\right)\left(1-M \frac{W_{t}}{P_{t}}\right)+\frac{G_{t}}{P_{t}(1-\varepsilon)}\right]=0
$$

Recall: $\Lambda_{t-1, t}=\beta \frac{C_{t-1}}{C_{t}}$

$$
\begin{aligned}
& \mathbb{E}_{t-1}\left[\left(Y_{t-1}-G_{t-1}\right)\left(1-M \frac{W_{t}}{P_{t}}\right)+\frac{G_{t}}{P_{t}(1-\varepsilon)}\right]=0 \\
& \mathbb{E}_{t-1}\left[\left(1-\gamma_{t-1}\right) Y_{t-1}\left(1-M\left(1-\gamma_{t}\right) N_{t}^{1+\varphi}\right)+\frac{\gamma_{t} Y_{t}}{P_{t}(1-\varepsilon)}\right]=0
\end{aligned}
$$
}
\end{enumerate}
}
