\section{Hayashi 2}

\subsection{Inference}

\begin{align*}
    t_j = \frac{\widehat{\beta}_j-\beta_j}{\operatorname{se}\left(\widehat{\beta}_j\right)} \\
    \beta^0 \in \widehat{\beta}_j \pm t_{n-K}^\alpha \operatorname{se}\left(\widehat{\beta}_j\right)
\end{align*}

\subsubsection{Linear restrictions}

\begin{align*}
    F &= \frac{\left(R^{\prime} \widehat{\beta}-r\right)^{\prime}\left[R^{\prime}\left(X^{\prime} X\right)^{-1} R\right]^{-1}\left(R^{\prime} \widehat{\beta}-r\right) / p}{\left((n-k) s^2 / \sigma^2\right) /(n-k)} \\
    &= \frac{\left(e^{\prime *} e^*-e^{\prime} e\right) / p}{e^{\prime} e /(n-K)}=\frac{\left(S S R^*-S S R\right) / p}{S S R /(n-K)} \\
    &= \frac{\left(R^2-R^{* 2}\right) / p}{\left(1-R^2\right) /(n-K)} =\frac{\left(S S T^*-S S R\right) / p}{S S R /(n-K)}
\end{align*}

$p$: number of regressors w/o constant \newline
$n-K$: number of individuals minus number of regressors with constant
\newline
last equation only for regression output useful

\subsubsection{Goodness of Fit}

\begin{align*}
    R^2&=\frac{\sum\left(\widehat{y}_i-\bar{y}\right)^2}{\sum\left(y_i-\bar{y}\right)^2}=M S S / T S S \\
    &=1-\frac{\sum e_i^2}{\sum\left(y_i-\bar{y}\right)^2}=1-(R S S / T S S) \\
    \hat{R}^2&=1-\frac{\sum e_i^2 /(n-K)}{\sum\left(y_i-\bar{y}\right)^2 /(n-1)} \\
    & = 1-\left(1-R^2\right) \frac{n-1}{n-k}
\end{align*}

\subsubsection{Wald Statistic}

$V(\widehat{\beta} \mid X)$ is given in outputs. Do not forget to square $\operatorname{SE}(\hat{\beta})$.

\begin{align*}
    W &=\left(R^{\prime} \widehat{\beta}-r\right)^{\prime}\left[R^{\prime} V(\widehat{\beta} \mid X) R\right]^{-1}\left(R^{\prime} \widehat{\beta}-r\right)\\
    &=n\left(R^{\prime} \widehat{\beta}-r\right)^{\prime}\left[R^{\prime} \hat{\operatorname{Avar}}(\widehat{\beta}) R\right]^{-1}\left(R^{\prime} \widehat{\beta}-r\right)\\
    W&=a(\hat{\beta})^{\prime}\left[\nabla a(\hat{\beta})^{\prime} \hat{V}(\hat{\beta}\mid X) \nabla a(\hat{\beta})\right]^{-1} a(\hat{\beta}) \\
    &= n a(\hat{\beta})^{\prime}\left[\nabla a(\hat{\beta})^{\prime} \hat{\operatorname{Avar}}(\hat{\beta}) \nabla a(\hat{\beta})\right]^{-1} a(\hat{\beta})
\end{align*}

